WIP: progress for write

theories/steps_progress.v
@@ -113,23 +113,153 @@ Proof.
     intros. by rewrite -(elem_of_dom (D:= gset loc) σ.(cheap)).
 Qed.
 
-Lemma copy_head_step σ l bor T
-  (BLK: ∀ n, (n < tsize T)%nat → l +ₗ n ∈ dom (gset loc) σ.(cheap)) :
+Lemma read_mem_is_Some l n h
+  (BLK: ∀ m, (m < n)%nat → l +ₗ m ∈ dom (gset loc) h) :
+  is_Some (read_mem l n h).
+Proof.
+  revert BLK.
+  eapply (read_mem_elim
+            (λ l n h ovl,
+              (∀ m : nat, (m < n)%nat → l +ₗ m ∈ dom (gset loc) h) → is_Some ovl)
+            (λ _ _ h l n oacc govl,
+              (∀ m : nat, (m < n)%nat → l +ₗ m ∈ dom (gset loc) h) →
+              is_Some oacc → is_Some govl)).
+  - naive_solver.
+  - naive_solver.
+  - intros l1 n1 h2 l2 n2 oacc IH BLK [acc Eqacc].
+    rewrite Eqacc /=.
+    assert (is_Some (h2 !! l2)) as [v2 Eq2].
+    { apply (elem_of_dom (D:=gset loc)). rewrite -(shift_loc_0_nat l2).
+      apply BLK. lia. }
+    rewrite Eq2 /=. apply IH; [|by eexists].
+    intros m Lt. rewrite shift_loc_assoc -(Nat2Z.inj_add 1). apply BLK. lia.
+Qed.
+
+Lemma read_mem_values l n h vl :
+  read_mem l n h = Some vl →
+  length vl = n ∧
+  (∀ i, (i < n)%nat → h !! (l +ₗ i) = vl !! i).
+Proof.
+  eapply (read_mem_elim
+            (λ l n h ovl, ∀ vl, ovl = Some vl →
+              length vl = n ∧
+              (∀ i, (i < n)%nat → h !! (l +ₗ i) = vl !! i))
+            (λ _ _ h l n oacc ovl, ∀ acc vl,
+              oacc = Some acc → ovl = Some vl →
+              (∀ i, (i < length acc)%nat → h !! (l +ₗ (i - length acc)) = acc !! i) →
+              length vl = (length acc + n)%nat ∧
+              (∀ i, (i < length acc)%nat → h !! (l +ₗ (i - length acc)) = vl !! i) ∧
+              (∀ i, (i < n)%nat → h !! (l +ₗ i) = vl !! (length acc + i)%nat))).
+  - intros ??? IH vl1 Eq.
+    destruct (IH [] vl1) as [IH1 IH2]; [done..|simpl;intros;lia|].
+    split; [done|]. intros i.
+     rewrite -{2}(Nat.add_0_l i) -(nil_length (A:=immediate)). by apply IH2.
+  - clear. intros __????????. simplify_eq. intros ?.
+    split; [lia|]. split; [done|intros; lia].
+  - clear. move => l0 n0 h l n oacc IH acc vl -> /=.
+    case lookup as [v|] eqn:Eq; [|done].
+    move => /= Eqvl ACC.
+    destruct (IH acc v (acc ++ [v]) vl eq_refl Eqvl) as [IH0 [IH1 IH2]];
+      last split; last split.
+    { intros i. rewrite app_length /=. intros Lt.
+      rewrite (_: l +ₗ 1 +ₗ (i - (length acc + 1)%nat) = l +ₗ (i - length acc));
+        last first. { rewrite shift_loc_assoc. f_equal. lia. }
+      case (decide (i = length acc)) => ?; [subst i|].
+      - by rewrite Z.sub_diag shift_loc_0 list_lookup_middle.
+      - have ?: (i < length acc)%nat by lia.
+        rewrite ACC; [|done]. by rewrite lookup_app_l. }
+    { rewrite IH0 app_length /=. lia. }
+    { intros i Lt. rewrite -IH1; [|rewrite app_length /=; lia].
+      f_equal. rewrite shift_loc_assoc. f_equal. rewrite app_length /=. lia. }
+    intros [|i] Lt.
+    + rewrite Nat.add_0_r -IH1; [|rewrite app_length /=; lia].
+      rewrite app_length /= shift_loc_assoc. do 2 f_equal. lia.
+    + rewrite (_: (l +ₗ S i) =  (l +ₗ 1 +ₗ i));
+        [|rewrite shift_loc_assoc; f_equal; lia].
+      rewrite IH2; [|lia]. f_equal. rewrite app_length /=. lia.
+Qed.
+
+Fixpoint borrow_read_match (β: barriers) (bor: borrow) (stack: list stack_item)
+  :=
+  match stack with
+  | [] => False
+  | Raw :: stack => True
+  | FnBarrier c :: stack => ¬ is_active β c ∧ borrow_read_match β bor stack
+  | Uniq t :: stack =>
+      bor = UniqB t ∨ bor ≠ UniqB t ∧ borrow_read_match β bor stack
+  end.
+
+Lemma access1'_read_progress bor stack β
+  (BOR: borrow_read_match β bor stack) :
+  ∃ stack', access1' stack bor AccessRead β = Some stack'.
+Proof.
+  induction stack as [|si stack IH]; [done|].
+  destruct si as [t1| |c]; [destruct bor as [t2|ot]|destruct bor|]; simpl;
+    [| |by eexists|by eexists|].
+  - destruct BOR as [Eq|[NEq BOR]].
+    + inversion Eq. rewrite decide_True; [by eexists|done].
+    + rewrite decide_False; [|naive_solver]. by apply IH.
+  - destruct BOR as [?|[? ?]]; [done|]. by apply IH.
+  - destruct BOR as [NB BOR]. rewrite /is_active bool_decide_false.
+    + by apply IH.
+    + intros ?. apply NB. by rewrite /is_active bool_decide_true.
+Qed.
+
+Lemma accessN_read_progress α β l bor (n: nat) :
+  (∀ m, (m < n)%nat → l +ₗ m ∈ dom (gset loc) α) →
+  (∀ (m: nat) stack, (m < n)%nat →
+    α !! (l +ₗ m) = Some stack →
+    is_Some stack.(frozen_since) ∨ borrow_read_match β bor stack.(borrows)) →
+  ∃ α', accessN α β l bor n AccessRead = Some α'.
+Proof.
+  revert α. induction n as [|n IHn]; intros α IN BOR; simpl; [by eexists|].
+  assert (is_Some (α !! (l +ₗ n))) as [stack Eq].
+  { apply (elem_of_dom (D:=gset loc)), IN. by lia. }
+  rewrite Eq /=.
+  have BM: is_Some stack.(frozen_since) ∨ borrow_read_match β bor stack.(borrows)
+    by apply (BOR n); [lia|done].
+  assert (is_Some (access1 β stack bor AccessRead)) as [stack' Eq2].
+  { rewrite /access1. case frozen_since as [tf|]; [by eexists|].
+    destruct BM as [?%is_Some_None|[? Eq']%access1'_read_progress]; [done|].
+    rewrite Eq'; by eexists. }
+  rewrite Eq2 /=. apply IHn.
+  - intros. apply elem_of_dom. rewrite lookup_insert_ne.
+    + apply (elem_of_dom (D:=gset loc)), IN. lia.
+    + move => /shift_loc_inj. lia.
+  - intros ???. rewrite lookup_insert_ne.
+    + apply BOR. lia.
+    + move => /shift_loc_inj. lia.
+Qed.
+
+Lemma copy_head_step (σ: state) l bor T
+  (WF: Wf σ)
+  (BLK: ∀ n, (n < tsize T)%nat → l +ₗ n ∈ dom (gset loc) σ.(cheap))
+  (BOR: ∀ m stack, (m < tsize T)%nat → σ.(cstk) !! (l +ₗ m) = Some stack →
+    is_Some stack.(frozen_since) ∨ borrow_read_match σ.(cbar) bor stack.(borrows)) :
   ∃ σ' vl,
   head_step (Copy (Place l bor T)) σ
             [CopyEvt l bor T vl] (of_val (TValV vl)) σ' [].
 Proof.
-  do 2 eexists. econstructor.
-  - econstructor.
-
-Abort.
+  destruct (read_mem_is_Some _ _ _ BLK) as [vl RM].
+  destruct (accessN_read_progress σ.(cstk) σ.(cbar) l bor (tsize T));[|done|].
+  { move => ? /BLK. by rewrite (state_wf_dom _ WF). }
+  do 2 eexists. econstructor; econstructor; [done..|].
+  move => l1 bor1 /elem_of_list_lookup [i Eqi].
+  apply (state_wf_mem_bor _ WF (l +ₗ i) l1).
+  destruct (read_mem_values _ _ _ _ RM) as [Eq1 Eq2].
+  rewrite Eq2; [done|]. rewrite -Eq1. by eapply lookup_lt_Some.
+Qed.
 
 Lemma write_head_step σ l bor T el vl
-  (VALUES: to_val (TVal el) = Some (TValV vl)) :
+  (LEN: length vl = tsize T)
+  (VALUES: to_val (TVal el) = Some (TValV vl))
+  (BLK: ∀ n, (n < tsize T)%nat → l +ₗ n ∈ dom (gset loc) σ.(cheap))
+  (LOCVAL: vl <<b σ.(cclk)) :
   ∃ σ',
   head_step (Write (Place l bor T) (TVal el)) σ
             [WriteEvt l bor T vl] #☠ σ' [].
 Proof.
+  eexists. econstructor; econstructor; [done|by rewrite LEN|done|..|done].
 Abort.
 
 Lemma deref_head_step σ l bor T mut :
@@ -150,9 +280,9 @@ Lemma endcall_head_step σ c (NZ: 0 ≤ c)
   head_step (EndCall #c) σ [EndCallEvt (Z.to_nat c)] #☠ σ' [].
 Proof. eexists. econstructor; econstructor. lia. done. Qed.
 
-Lemma retag_head_step σ x xbor T kind :
-  ∃ σ',
-  head_step (Retag (Place x xbor T) kind) σ [RetagEvt x T kind] #☠ σ' [].
+Lemma retag_head_step σ x xbor T kind call :
+  ∃ σ' kind',
+  head_step (Retag (Place x xbor T) kind call) σ [RetagEvt x T kind'] #☠ σ' [].
 Proof.
 Abort.
 
